For inter to pyramid synapse.
\subsection{First for Delta}
Here $V_{o}$ means voltage in the apical compartment for the post-synaptic neuron and $r_{i}$ the output rate (on the previous time step) for the pre-synaptic neuron.
\begin{eqnarray}
  \dot{\delta} = -\frac{1}{\tau}\left(\delta + V_{o} r_{i}\right)\\
  \dot{\delta} + \frac{1}{\tau}\delta = -\frac{1}{\tau} V_{o} r_{i}
\end{eqnarray}
This is a `standard' first-order ordinary differential equation so we use integrating factor $e^{t/\tau}$.
\begin{eqnarray}
  \dot{\delta}e^{t/\tau} + \frac{1}{\tau}\delta e^{t/\tau} &=& -\frac{1}{\tau} e^{t/\tau}V_{o} r_{i} \\
\end{eqnarray}
To fit into product rule for derivatives $\left[(f\cdot g)' = f\cdot g' + g\cdot f'\right]$
\begin{eqnarray}
f = e^{t/\tau} &\text{ and }& \dot{h} = \dot{\delta}\\
\dot{f} = \frac{1}{\tau} e^{t/\tau}  &\text{ and }& h = \delta
\end{eqnarray}
we now get
\begin{equation}
\left(\delta e^{t/\tau}\right)' = -\frac{1}{\tau} e^{t/\tau} V_{o} r_{i} 
\end{equation}
Integrating both sides
\begin{eqnarray}
\delta e^{t/\tau} &=& -V_{o} r_{i} \int_{0}^{t} \frac{1}{\tau} e^{t/\tau} dt \\
    &=& -V_{o} r_{i} \left[e^{t/\tau}\right]_{0}^{t} + C\\
    &=& -V_{o} r_{i} \left[e^{t/\tau} - 1\right] + C \\
\delta &=& \left[-V_{o} r_{i} \left(e^{t/\tau} - 1\right) + C \right] e^{-t/\tau}\\
\delta &=& -V_{o} r_{i} \left(1 - e^{-t/\tau} \right) + Ce^{-t/\tau}
\label{delta_at_t_with_C}
\end{eqnarray}
To find $C$ and, since we want to integrate between spikes, we'll calculate the constant at $t_k$ (last time at which pre-synaptic spiked). $\delta_k$ is the value of $\delta$ at time $t_k$.
\begin{eqnarray}
C &=& \left[\delta_k + V_{o} r_{i} \left(1 - e^{-t_k/\tau} \right)\right] e^{t_k/\tau}
\label{C_for_delta_at_k}
\end{eqnarray}
Substituting \ref{C_for_delta_at_k} in \ref{delta_at_t_with_C}

\begin{eqnarray}
\delta &=& -V_{o} r_{i} \left(1 - e^{-t/\tau} \right) + \left[\delta_k + V_{o} r_{i} \left(1 - e^{-t_k/\tau} \right)\right] e^{t_k/\tau}e^{-t/\tau}
\end{eqnarray}
Let $\Delta t = t - t_k$

\begin{eqnarray}
\delta &=& -V_{o} r_{i} \left(1 - e^{-t/\tau} \right) + \delta_k e^{-\Delta t/\tau}+ V_{o} r_{i} \left(e^{t_k/\tau} - 1\right)e^{-t/\tau}\\
\delta &=& -V_{o} r_{i} + \cancel{V_{o} r_{i} e^{-t/\tau}} + \delta_k e^{-\Delta t/\tau}+ V_{o} r_{i} e^{-\Delta t/\tau} - \cancel{V_{o} r_{i} e^{-t/\tau}}
\end{eqnarray}
Finally
\begin{eqnarray}
\delta &=& -V_{o} r_{i} \left(1 - e^{-\Delta t/\tau}\right)  + \delta_k e^{-\Delta t/\tau}
\end{eqnarray}

\subsection{Now for efficacy}
We'll use the same notation as before $V_{o} = V^{apical}_{post}$ and $r_{i} = r_{pre}$.
\begin{eqnarray}
	\dot{g} &=& \eta \delta \\
	\int\dot{g} &=& \eta \int\delta dt\\	
	g &=& \eta \int \left[ -V_{o} r_{i} \left(1 - e^{-\Delta t/\tau}\right)  + \delta_k e^{-\Delta t/\tau} \right]dt \\
	g &=& \eta \left[ -V_{o} r_{i} \left(t + \tau e^{-\Delta t/\tau}\right)  - \delta_k \tau e^{-\Delta t/\tau} \right] + C
	\label{eq:g-at-t}
\end{eqnarray}
Obtain the constant at time $t_k$, remember that $\Delta t = t - t_k$
\begin{eqnarray}
	C &=& g_{k} + \eta \left[ V_{o} r_{i} \left(t + \tau e^{-\Delta t/\tau}\right) + \delta_k \tau e^{-\Delta t/\tau} \right]\\
	C &=& g_{k} + \eta \left[ V_{o} r_{i} \left(t_{k} + \tau\right) + \delta_k \tau \right]
	\label{eq:gk}
\end{eqnarray}
Now substituting \ref{eq:gk} in \ref{eq:g-at-t}
\begin{eqnarray}
	g &=& \eta \left[ -V_{o} r_{i} \left(t + \tau e^{-\Delta t/\tau}\right)  - \delta_k \tau e^{-\Delta t/\tau} \right] +  \nonumber\\
	& & g_{k} + \eta \left[ V_{o} r_{i} \left(t_{k} + \tau\right) + \delta_k \tau \right]\\
	&=& g_{k} -\eta \left[V_{o} r_{i} \left(t_{k} + \tau - t - \tau e^{-\Delta t/\tau}\right)  -  \right. \nonumber\\
    & & \left. \delta_k \tau e^{-\Delta t/\tau} + \delta_k \tau\right] \\
	&=& g_{k} -\eta \left[V_{o} r_{i} \left(-\Delta t + \tau\left[1 - e^{-\Delta t/\tau}\right]\right)  +  \right. \nonumber\\
    & & \left. \delta_k \tau\left(1 - e^{-\Delta t/\tau} \right)\right]
\end{eqnarray}
Let $\gamma = 1 - e^{-\Delta t/\tau}$
\begin{eqnarray}
	g &=& g_{k} -\eta \left[V_{o} r_{i} \left(-\Delta t + \tau\gamma\right)  + 
          \delta_k \tau \gamma \right] \\
g &=& g_{k} -\eta \tau \left[V_{o} r_{i} \left(\gamma -\frac{\Delta t}{\tau} \right)  + 
\delta_k \gamma \right] 
\end{eqnarray}


